src/Dafny/bitwiseBinaryOperations.i.dfy
@@ -1,0 +1,311 @@
+include "ops.dfy"
+include "types.dfy"
+include "conversionOperations.i.dfy"
+
+// Contains the following bitwise binary operations: LSHL, AND, OR
+module bitwise_binary_operations_i {
+    import opened ops
+    import opened types
+    import opened conversion_operations_i
+
+    // TODO: REWRITE WITH BINOPS
+     function evalLSHR(op1:Data,op2:Data): (out:Data) // still wip
+        requires isInt(op1) && isInt(op2)
+        requires op1.itype.size*8 > op2.val //See note above
+        requires op2.val > 0
+        ensures out.Int?;
+        ensures out.itype.size == op1.itype.size && !out.itype.signed;
+     {
+        reveal_IntFits();
+        reveal_rightShift();
+        var initial := if op1.itype.signed then ToTwosComp(op1).val else op1.val;
+        var result := rightShift(initial,op2.val);
+        ValToData(result,op1.itype.size,false)
+
+     }
+    function {:opaque} rightShift(val:int,shift:int) : (result:int)
+        requires shift >= 1
+        requires val >= 0
+        ensures result <= val
+        ensures result >= 0
+        decreases shift
+    {
+        var r:real := (val/2) as real;
+        if shift == 1 then r.Floor
+        else  rightShift(r.Floor,shift-1)
+    }
+
+    function evalAND(dstSize:bitWidth,op1:Data,op2:Data): (out:Data)
+        requires isInt(op1) && isInt(op2)
+        requires typesMatch(op1,op2)
+        requires dstSize == op1.itype.size
+        ensures out.Int?;
+        ensures out.itype.size == dstSize && !out.itype.signed;
+    {
+        reveal_BitAnd();
+        reveal_BitsToWord();
+        reveal_WordToBits();
+        if dstSize == 1 then evalAND8(dstSize,op1,op2) else 
+        if dstSize == 2 then evalAND16(dstSize,op1,op2) else 
+        if dstSize == 4 then evalAND32(dstSize,op1,op2) else 
+        evalAND64(dstSize,op1,op2) 
+
+    }
+
+    function evalOR(dstSize:bitWidth,op1:Data,op2:Data): (out:Data)
+        requires isInt(op1) && isInt(op2)
+        requires typesMatch(op1,op2)
+        requires dstSize == op1.itype.size
+        ensures out.Int?
+        ensures out.itype.size == dstSize && !out.itype.signed
+    {
+        reveal_BitOr();
+        reveal_BitsToWord();
+        reveal_WordToBits();
+        if dstSize == 1 then evalOR8(dstSize,op1,op2) else 
+        if dstSize == 2 then evalOR16(dstSize,op1,op2) else 
+        if dstSize == 4 then evalOR32(dstSize,op1,op2) else 
+        evalOR64(dstSize,op1,op2) 
+
+    }
+/// HELPER FUNCTIONS
+    // AND HELPER FUNCTIONS //
+function evalAND8(dstSize:bitWidth,op1:Data,op2:Data): (out:Data)
+      requires isInt(op1) && isInt(op2)
+      requires typesMatch(op1,op2)
+      requires op1.itype.size == 1
+      requires dstSize == op1.itype.size
+      ensures out.Int?;
+      ensures out.itype.size == dstSize && !out.itype.signed;
+     {
+        reveal_ToTwosComp(); 
+        reveal_IntFits();
+        var result := BitwiseAndBytes(ToTwosComp(op1).val,ToTwosComp(op2).val);
+        ValToData(result,1,false)      
+     }     
+
+function evalAND16(dstSize:bitWidth,op1:Data,op2:Data): (out:Data)
+      requires isInt(op1) && isInt(op2)
+      requires typesMatch(op1,op2)
+      requires op1.itype.size == 2
+      requires dstSize == op1.itype.size
+      ensures out.Int?;
+      ensures out.itype.size == dstSize && !out.itype.signed;
+     {
+        reveal_ToTwosComp(); 
+        reveal_IntFits();
+        var result := BitwiseAndHalfWord(ToTwosComp(op1).val,ToTwosComp(op2).val);
+        ValToData(result,2,false)      
+     }
+
+function evalAND32(dstSize:bitWidth,op1:Data,op2:Data): (out:Data)
+      requires isInt(op1) && isInt(op2)
+      requires typesMatch(op1,op2)
+      requires op1.itype.size == 4
+      requires dstSize == op1.itype.size
+      ensures out.Int?;
+      ensures out.itype.size == dstSize && !out.itype.signed;
+     {
+        reveal_ToTwosComp(); 
+        reveal_IntFits();
+        var result := BitwiseAnd(ToTwosComp(op1).val,ToTwosComp(op2).val);
+        ValToData(result,4,false)      
+     }
+
+function evalAND64(dstSize:bitWidth,op1:Data,op2:Data): (out:Data)
+      requires isInt(op1) && isInt(op2)
+      requires typesMatch(op1,op2)
+      requires op1.itype.size == 8
+      requires dstSize == op1.itype.size
+      ensures out.Int?;
+      ensures out.itype.size == dstSize && !out.itype.signed;
+     {
+        reveal_ToTwosComp(); 
+        reveal_IntFits();
+        var result := BitwiseAnd64(ToTwosComp(op1).val,ToTwosComp(op2).val);
+        ValToData(result,8,false)      
+     }
+
+    // OR HELPER FUNCTIONS //
+function evalOR8(dstSize:bitWidth,op1:Data,op2:Data): (out:Data)
+      requires isInt(op1) && isInt(op2)
+      requires typesMatch(op1,op2)
+      requires op1.itype.size == 1
+      requires dstSize == op1.itype.size
+      ensures out.Int?;
+      ensures out.itype.size == dstSize && !out.itype.signed;
+     {
+        reveal_ToTwosComp(); 
+        reveal_IntFits();
+        var result := BitwiseOrBytes(ToTwosComp(op1).val,ToTwosComp(op2).val);
+        ValToData(result,1,false)      
+     }     
+
+function evalOR16(dstSize:bitWidth,op1:Data,op2:Data): (out:Data)
+      requires isInt(op1) && isInt(op2)
+      requires typesMatch(op1,op2)
+      requires op1.itype.size == 2
+      requires dstSize == op1.itype.size
+      ensures out.Int?;
+      ensures out.itype.size == dstSize && !out.itype.signed;
+     {
+        reveal_ToTwosComp(); 
+        reveal_IntFits();
+        var result := BitwiseOrHalfWord(ToTwosComp(op1).val,ToTwosComp(op2).val);
+        ValToData(result,2,false)      
+     }
+
+function evalOR32(dstSize:bitWidth,op1:Data,op2:Data): (out:Data)
+      requires isInt(op1) && isInt(op2)
+      requires typesMatch(op1,op2)
+      requires op1.itype.size == 4
+      requires dstSize == op1.itype.size
+      ensures out.Int?;
+      ensures out.itype.size == dstSize && !out.itype.signed;
+     {
+        reveal_ToTwosComp(); 
+        reveal_IntFits();
+        var result := BitwiseOr(ToTwosComp(op1).val,ToTwosComp(op2).val);
+        ValToData(result,4,false)      
+     }
+
+function evalOR64(dstSize:bitWidth,op1:Data,op2:Data): (out:Data)
+      requires isInt(op1) && isInt(op2)
+      requires typesMatch(op1,op2)
+      requires op1.itype.size == 8
+      requires dstSize == op1.itype.size
+      ensures out.Int?;
+      ensures out.itype.size == dstSize && !out.itype.signed;
+     {
+        reveal_ToTwosComp(); 
+        reveal_IntFits();
+        var result := BitwiseOr64(ToTwosComp(op1).val,ToTwosComp(op2).val);
+        ValToData(result,8,false)      
+     }
+     // --  Lemmas for correctness checking -----
+    lemma evalSHLIsValid()
+    {
+       
+    }
+
+    lemma evalLSHRIsValid()
+    {
+        reveal_IntFits();
+        reveal_IntFromBytes();
+        reveal_IntToBytes();
+        reveal_ExtendZeroBytes();
+        reveal_rightShift();
+        reveal_WordToBits64();
+        reveal_BitsToWord64();
+        reveal_ToTwosComp();
+        // <result> = lshr i32 4, 1   ; yields i32:result = 2
+         var v0:uint32 := 4;
+         var v1:uint32 := 1;
+         var d0:uint32 := 2;
+         var out:Data := evalLSHR(UInt32(v0),UInt32(v1));
+         assert out.itype.size == 4;// == UInt64(d0);
+         assert out.val == 2;
+         assert out.val == UInt32(d0).val;
+
+        // <result> = lshr i32 4, 2   ; yields i32:result = 1
+         var v2:uint32 := 4;
+         var v3:uint32 := 2;
+         var d1:uint32 := 1;
+         var out1:Data := evalLSHR(UInt32(v2),UInt32(v3));
+         assert out1.itype.size == 4;// == UInt64(d0);
+         assert out1.val == 1;
+         assert out1.val == UInt32(d1).val;
+
+        // <result> = lshr i8  4, 3   ; yields i8:result = 0
+         var v4:uint32 := 4;
+         var v5:uint32 := 3;
+         var d2:uint32 := 0;
+         var out2:Data := evalLSHR(UInt32(v4),UInt32(v5));
+         assert out2.itype.size == 4;// == UInt64(d0);
+         assert out2.val == 0;
+         assert out2.val == UInt32(d2).val;
+         
+        // <result> = lshr i8 -2, 1   ; yields i8:result = 0x7F
+         var v6:sint8 := -2;
+         var v7:uint32 := 1;
+         var d3:uint8 := 127;
+         var out3:Data := evalLSHR(SInt8(v6),UInt32(v7));
+         assert out3.itype.size == 1;// == UInt64(d0);
+         assert out3.val == 127;
+         assert out3.val == UInt8(d3).val;
+
+         // <result> = lshr i8 -2, 1   ; yields i8:result = 0x7F
+         var v8:sint8 := -42;
+         var v9:uint32 := 2;
+         var d4:uint8 := 53;
+         var out4:Data := evalLSHR(SInt8(v8),UInt32(v9));
+         assert out4.itype.size == 1;// == UInt64(d0);
+         assert out4.val == 53;
+         assert out4.val == UInt8(d4).val;
+
+        //
+       
+    }
+
+    lemma evalANDIsValid()
+    {
+         reveal_BitAnd();
+         reveal_BitAnd16();
+         reveal_BitAnd8();
+         reveal_BitAnd64();
+         reveal_BitsToWord();
+         reveal_WordToBits();
+
+        //<result> = and i32 15, 40     ; yields i32:result = 8
+         var v0:uint32 := 15;
+         var v1:uint32 := 40;
+         var d0:uint32 := 8;
+         var out:Data := evalAND(4,UInt32(v0),UInt32(v1));
+         assert out.itype.size == 4;// == UInt64(d0);
+         lemma_WordToBitsToWord(v0);
+         assert WordToBits(v0) == 15;
+         assert WordToBits(v1) == 40;
+         assert out.val == 8;
+        // <result> = and i32 4, 8      ; yields i32:result = 0
+         var v2:uint32 := 4;
+         var v3:uint32 := 8;
+         var d1:uint32 := 8;
+         var out1:Data := evalAND(4,UInt32(v2),UInt32(v3));
+         assert out1.itype.size == 4;// == UInt64(d0);
+         assert WordToBits(v2) == 4;
+         assert WordToBits(v3) == 8;
+         assert out1.val == 0;
+
+    }
+
+        lemma evalORIsValid()
+    {
+         reveal_BitOr();
+         reveal_BitOr16();
+         reveal_BitOr8();
+         reveal_BitOr64();
+         reveal_BitsToWord();
+         reveal_WordToBits();
+
+        //<result> = and i32 15, 40     ; yields i32:result = 47
+         var v0:uint32 := 15;
+         var v1:uint32 := 40;
+         var out:Data := evalOR(4,UInt32(v0),UInt32(v1));
+         assert out.itype.size == 4;// == UInt64(d0);
+         lemma_WordToBitsToWord(v0);
+         assert WordToBits(v0) == 15;
+         assert WordToBits(v1) == 40;
+         assert out.val == 47;
+        // <result> = and i32 4, 8      ; yields i32:result = 12
+         var v2:uint32 := 4;
+         var v3:uint32 := 8;
+         var out1:Data := evalOR(4,UInt32(v2),UInt32(v3));
+         assert out1.itype.size == 4;// == UInt64(d0);
+         assert WordToBits(v2) == 4;
+         assert WordToBits(v3) == 8;
+         assert out1.val == 12;
+
+    }
+
+
+}
